Weidenbach_Book/CDCL_Two_Watched_Literals_Implementation.thy
@@ -5,7 +5,7 @@
 subsection \<open>Implementation for 2 Watched-Literals\<close>
 
 theory CDCL_Two_Watched_Literals_Implementation
-imports CDCL_Two_Watched_Literals
+imports CDCL_W_Abstract_State
 begin
 text \<open>The difference between an implementation and the core described in the previous sections are
   the following:
@@ -35,23 +35,21 @@ text \<open>It is important to remember that a conflicting clause with respect t
   finish updating the data-structure (both to keep the invariant and find a potentially better
   conflict). A conflict is better when it involves less literals, i.e.\ less propagations are needed
   before finding the conflict.\<close>
-datatype 'v candidate =
+(* datatype 'v candidate =
   Prop_Or_Conf
     (prop_queue: "('v literal \<times> 'v literal list twl_clause) list")
-    (conflict: "'v twl_clause option")
+    (conflict: "'v twl_clause option") *)
 
-fun twl_clause_to_mset where
-"twl_clause_to_mset (TWL_Clause W UW) = TWL_Clause (mset W) (mset UW)"
+datatype 'v twl_clause =
+  TWL_Clause (watched: 'v) (unwatched: 'v)
 
 locale raw_clss_with_update =
-  raw_clss cls_lit in_cls mset_cls clss_cls in_clss mset_clss
+  raw_clss get_lit mset_cls get_cls mset_clss
   for
-    cls_lit :: "'cls \<Rightarrow> 'lit \<Rightarrow> 'v literal" and
-    in_cls :: "'lit \<Rightarrow> 'cls \<Rightarrow> bool" and
+    get_lit :: "'cls \<Rightarrow> 'lit \<Rightarrow> 'v literal option" and
     mset_cls :: "'cls \<Rightarrow> 'v clause" and
 
-    clss_cls :: "'clss \<Rightarrow> 'cls_it \<Rightarrow> 'cls" and
-    in_clss :: "'cls_it \<Rightarrow> 'clss \<Rightarrow> bool" and
+    get_cls :: "'clss \<Rightarrow> 'cls_it \<Rightarrow> 'cls option" and
     mset_clss:: "'clss \<Rightarrow> 'cls multiset" +
   fixes
     twl_cls :: "'cls \<Rightarrow> 'v literal list twl_clause" and
@@ -80,11 +78,11 @@ begin
 
 end
 
-locale twl_state\<^sub>W_clss_ops =
+locale twl_state\<^sub>W_clss =
   abs_state\<^sub>W
     \<comment> \<open>functions for clauses: \<close>
-    cls_lit in_cls mset_cls
-    clss_cls in_clss mset_clss
+    get_lit mset_cls
+    get_cls mset_clss
 
     \<comment> \<open>functions for the conflicting clause:\<close>
     mset_ccls
@@ -102,8 +100,126 @@ locale twl_state\<^sub>W_clss_ops =
     conc_init_state
     restart_state
     +
-  raw_clss_with_update cls_lit in_cls mset_cls clss_cls in_clss mset_clss twl_cls clss_update
-    swap_lit  exists_in_unwatched
+  raw_clss_with_update get_lit mset_cls get_cls mset_clss twl_cls clss_update
+    swap_lit exists_in_unwatched
+  for
+    \<comment> \<open>Clause:\<close>
+    get_lit :: "'cls \<Rightarrow> 'lit \<Rightarrow> 'v literal option" and
+    mset_cls :: "'cls \<Rightarrow> 'v clause" and
+
+    \<comment> \<open>Multiset of Clauses:\<close>
+    get_cls :: "'clss \<Rightarrow> 'cls_it \<Rightarrow> 'cls option" and
+    mset_clss:: "'clss \<Rightarrow> 'cls multiset" and
+
+    \<comment> \<open>Conflicting clause:\<close>
+    mset_ccls :: "'ccls \<Rightarrow> 'v clause" and
+
+    \<comment> \<open>2 watched literals conversion:\<close>
+    twl_cls :: "'cls \<Rightarrow> 'v literal list twl_clause" and
+    clss_update :: "'clss \<Rightarrow> 'cls_it \<Rightarrow> 'cls \<Rightarrow> 'clss" and
+    swap_lit :: "'cls \<Rightarrow> 'lit \<Rightarrow> 'lit \<Rightarrow> 'cls" and
+    exists_in_unwatched :: "('lit \<Rightarrow> bool) \<Rightarrow> 'cls \<Rightarrow> 'lit option" and
+    conc_trail :: "'st \<Rightarrow> ('v, 'v clause) ann_lits" and
+    hd_raw_conc_trail :: "'st \<Rightarrow> ('v, 'cls_it) ann_lit" and
+    raw_clauses :: "'st \<Rightarrow> 'clss" and
+    conc_backtrack_lvl :: "'st \<Rightarrow> nat" and
+    raw_conc_conflicting :: "'st \<Rightarrow> 'ccls option" and
+
+    conc_learned_clss :: "'st \<Rightarrow> 'v clauses" and
+
+    cons_conc_trail :: "('v, 'cls_it) ann_lit \<Rightarrow> 'st \<Rightarrow> 'st" and
+    tl_conc_trail :: "'st \<Rightarrow> 'st" and
+    add_conc_confl_to_learned_cls :: "'st \<Rightarrow> 'st" and
+    conc_remove_cls :: "'cls \<Rightarrow> 'st \<Rightarrow> 'st" and
+    update_conc_backtrack_lvl :: "nat \<Rightarrow> 'st \<Rightarrow> 'st" and
+    mark_conflicting :: "'cls_it \<Rightarrow> 'st \<Rightarrow> 'st" and
+    reduce_conc_trail_to :: "('v, 'v clause) ann_lits \<Rightarrow> 'st \<Rightarrow> 'st" and
+    resolve_conflicting :: "'v literal \<Rightarrow> 'cls \<Rightarrow> 'st \<Rightarrow> 'st" and
+
+    conc_init_state :: "'clss \<Rightarrow> 'st" and
+    restart_state :: "'st \<Rightarrow> 'st" +
+  fixes 
+    prop_queue :: "'st \<Rightarrow> ('v, 'v clause) ann_lits" and
+    cons_prop_queue :: "('v, 'cls_it) ann_lit \<Rightarrow> 'st \<Rightarrow> 'st" and
+    hd_prop_queue_to_trail :: "'st \<Rightarrow> 'st" and
+    prop_queue_to_trail :: "'st \<Rightarrow> 'st" and
+
+    get_undecided_lit :: "'st \<Rightarrow> 'v literal option" and
+    get_clause_watched_by :: "'st \<Rightarrow> 'v literal \<Rightarrow> 'cls_it list" and
+    update_clause :: "'st \<Rightarrow> 'cls_it \<Rightarrow> 'cls \<Rightarrow> 'st"
+  assumes
+    state_cons_prop_queue:
+      "undefined_lit (conc_trail T @ prop_queue T) (lit_of L) \<Longrightarrow>
+        state (cons_prop_queue L T) = state T" and
+    cons_prop_queue_prop_queue:
+      "undefined_lit (conc_trail T @ prop_queue T) (lit_of L) \<Longrightarrow>
+         prop_queue (cons_prop_queue L T) = mmset_of_mlit (raw_clauses T) L # prop_queue T" and
+    hd_prop_queue_to_trail_state:
+      "prop_queue T \<noteq> [] \<Longrightarrow> 
+        state T = (M, N, U, k, C) \<Longrightarrow>
+        state (hd_prop_queue_to_trail T) = 
+           (hd (prop_queue T) # M, N, U, k, C)" and
+    hd_prop_queue_to_trail:
+      "prop_queue T \<noteq> [] \<Longrightarrow> 
+        prop_queue (hd_prop_queue_to_trail T) = 
+           tl (prop_queue T)" and
+    prop_queue_to_trail_state:
+      "state T = (M, N, U, k, C) \<Longrightarrow>
+        state (prop_queue_to_trail T) = (prop_queue (prop_queue_to_trail T) @ M, N, U, k, C)" and
+    prop_queue_to_trail:
+      "prop_queue (prop_queue_to_trail T) = []" and
+      
+    get_undecided_lit_Some:
+      "get_undecided_lit T = Some L' \<Longrightarrow> undefined_lit (conc_trail T) L' \<and>
+        atm_of L' \<in> atms_of_mm (conc_clauses T)" and
+    get_undecided_lit_None:
+      "get_undecided_lit T = None \<longleftrightarrow>
+         (\<forall>L'. atm_of L' \<in> atms_of_mm (conc_clauses T) \<longrightarrow> \<not>undefined_lit (conc_trail T) L')" and
+    get_clause_watched_by:
+      "i \<in> set (get_clause_watched_by T K) \<longleftrightarrow> K \<in> set (watched (twl_cls (raw_clauses T \<Down> i)))" and
+    get_clause_watched_by_distinct:
+      "distinct (get_clause_watched_by T K)" and
+    update_clause:
+      "raw_clauses (update_clause S i E) = (raw_clauses S) (i := E)"
+
+locale abs_conflict_driven_clause_learning\<^sub>W_clss =
+  twl_state\<^sub>W_clss
+    \<comment> \<open>functions for clauses: \<close>
+    cls_lit in_cls mset_cls
+    clss_cls in_clss mset_clss
+
+    \<comment> \<open>functions for the conflicting clause:\<close>
+    mset_ccls
+    
+    twl_cls clss_update swap_lit  exists_in_unwatched
+    \<comment> \<open>functions about the state:\<close>
+      \<comment> \<open>getter:\<close>
+    conc_trail hd_raw_conc_trail raw_clauses conc_backtrack_lvl
+    raw_conc_conflicting conc_learned_clss
+      \<comment> \<open>setter:\<close>
+    cons_conc_trail tl_conc_trail add_conc_confl_to_learned_cls conc_remove_cls
+    update_conc_backtrack_lvl
+    mark_conflicting reduce_conc_trail_to resolve_conflicting
+
+      \<comment> \<open>Some specific states:\<close>
+    conc_init_state
+    restart_state
+    
+      -- \<open>Additional functions:\<close>
+        -- \<open>Propagate queue\<close>
+    prop_queue
+    cons_prop_queue 
+    hd_prop_queue_to_trail 
+    prop_queue_to_trail 
+    
+        -- \<open>Not decided literals\<close>
+    get_undecided_lit 
+
+        -- \<open>Watched clauses:\<close>
+    get_clause_watched_by
+    
+    update_clause
+  
   for
     \<comment> \<open>Clause:\<close>
     cls_lit :: "'cls \<Rightarrow> 'lit \<Rightarrow> 'v literal" and
@@ -140,841 +256,40 @@ locale twl_state\<^sub>W_clss_ops =
     reduce_conc_trail_to :: "('v, 'v clause) ann_lits \<Rightarrow> 'st \<Rightarrow> 'st" and
     resolve_conflicting :: "'v literal \<Rightarrow> 'cls \<Rightarrow> 'st \<Rightarrow> 'st" and
 
+    conc_init_state :: "'clss \<Rightarrow> 'st" and
+    restart_state :: "'st \<Rightarrow> 'st" and
+
     prop_queue :: "'st \<Rightarrow> ('v, 'v clause) ann_lits" and
     cons_prop_queue :: "('v, 'cls_it) ann_lit \<Rightarrow> 'st \<Rightarrow> 'st" and
     hd_prop_queue_to_trail :: "'st \<Rightarrow> 'st" and
     prop_queue_to_trail :: "'st \<Rightarrow> 'st" and
 
     get_undecided_lit :: "'st \<Rightarrow> 'v literal option" and
+    get_clause_watched_by :: "'st \<Rightarrow> 'v literal \<Rightarrow> 'cls_it list" and
+    update_clause :: "'st \<Rightarrow> 'cls_it \<Rightarrow> 'cls \<Rightarrow> 'st"
+begin
+
+fun other_watched_lit  where
+"other_watched_lit S i L =
+  (case remove1 L (watched (twl_cls (raw_clauses S \<Down> i))) of
+     [] \<Rightarrow> None
+   | a # _ \<Rightarrow> Some a)"
+
+fun update_clause where
+"update_clause L S i =
+  (case other_watched_lit S i L of
+     None \<Rightarrow> S
+   | Some L' \<Rightarrow>
+     if L' \<in> lits_of_l (conc_trail S)
+     then S
+     else
+       (case exists_in_unwatched 
+         (\<lambda>j. undefined_lit (conc_trail S) ((raw_clauses S \<Down> i) \<down> j)) (raw_clauses S \<Down> i) of
+         None \<Rightarrow> mark_conflicting i S
+       | Some _ \<Rightarrow> S)
+     )"
+     
+end
 
-    conc_init_state :: "'clss \<Rightarrow> 'st" and
-    restart_state :: "'st \<Rightarrow> 'st" +
-  assumes
-    state_cons_prop_queue:
-      "undefined_lit (conc_trail T @ prop_queue T) (lit_of L) \<Longrightarrow>
-        state (cons_prop_queue L T) = state T" and
-    cons_prop_queue_prop_queue:
-      "undefined_lit (conc_trail T @ prop_queue T) (lit_of L) \<Longrightarrow>
-         prop_queue (cons_prop_queue L T) = mmset_of_mlit (raw_clauses T) L # prop_queue T" and
-    hd_prop_queue_to_trail_state:
-      "prop_queue T \<noteq> [] \<Longrightarrow> 
-        state T = (M, N, U, k, C) \<Longrightarrow>
-        state (hd_prop_queue_to_trail T) = 
-           (hd (prop_queue T) # M, N, U, k, C)" and
-    hd_prop_queue_to_trail:
-      "prop_queue T \<noteq> [] \<Longrightarrow> 
-        prop_queue (hd_prop_queue_to_trail T) = 
-           tl (prop_queue T)" and
-    prop_queue_to_trail_state:
-      "state T = (M, N, U, k, C) \<Longrightarrow>
-        state (prop_queue_to_trail T) = (prop_queue (prop_queue_to_trail T) @ M, N, U, k, C)" and
-    prop_queue_to_trail:
-      "prop_queue (prop_queue_to_trail T) = []" and
-      
-    get_undecided_lit_Some:
-      "get_undecided_lit T = Some L' \<Longrightarrow> undefined_lit (conc_trail T) L' \<and>
-        atm_of L' \<in> atms_of_mm (conc_clauses T)" and
-    get_undecided_lit_None:
-      "get_undecided_lit T = None \<longleftrightarrow>
-         (\<forall>L'. atm_of L' \<in> atms_of_mm (conc_clauses T) \<longrightarrow> \<not>undefined_lit (conc_trail T) L')"
-
-      
-text \<open>Morally instead of @{typ "('v literal \<times> 'v twl_clause) list"}, we should use
-  @{typ "('v, 'v twl_clause) ann_lits"} with only @{term Propagated}. However, we do not
-  want to define the function for @{term Decided} too. The following function makes the conversion
-  from the pair to the trail:
-  \<close>
-abbreviation get_trail_of_cand where
-"get_trail_of_cand C \<equiv> map (case_prod Propagated) (prop_queue C)"
-
-datatype 'v twl_state_cands =
-  TWL_State_Cand (twl_state: "'v twl_state")
-    (cand: "'v candidate")
-
-fun raw_cons_trail where
-"raw_cons_trail L (TWL_State M N U k C) = TWL_State (L # M) N U k C"
-
-lemma raw_init_clss_raw_cons_trail[simp]:
-  "raw_init_clss (raw_cons_trail L T) = raw_init_clss T"
-  by (cases T) auto
-
-lemma raw_learned_clss_raw_cons_trail[simp]:
-  "raw_learned_clss (raw_cons_trail L T) = raw_learned_clss T"
-  by (cases T) auto
-
-lemma length_raw_trail_raw_cons_trails[simp]:
-  "length (raw_trail (raw_cons_trail L S)) = Suc (length (raw_trail S))"
-  by (cases S) auto
-
-lemma twl_raw_clauses_raw_cons_trail[simp]:
-  "raw_clauses_of_twl (raw_cons_trail L S) = raw_clauses_of_twl S"
-  by (cases S) auto
-
-fun raw_prepend_trail where
-"raw_prepend_trail Ms (TWL_State M N U k C) = TWL_State (Ms @ M) N U k C"
-
-lemma raw_init_clss_raw_prepend_trail[simp]:
-  "raw_init_clss (raw_prepend_trail L T) = raw_init_clss T"
-  by (cases T) auto
-
-lemma raw_learned_clss_raw_prepend_trail[simp]:
-  "raw_learned_clss (raw_prepend_trail L T) = raw_learned_clss T"
-  by (cases T) auto
-
-lemma length_raw_trail_raw_prepend_trails[simp]:
-  "length (raw_trail (raw_prepend_trail L S)) = length L + length (raw_trail S)"
-  by (cases S) auto
-
-lemma twl_raw_clauses_raw_prepend_trail[simp]:
-  "raw_clauses_of_twl (raw_prepend_trail L S) = raw_clauses_of_twl S"
-  by (cases S) auto
-
-fun raw_cons_trail_pq where
-"raw_cons_trail_pq L (TWL_State_Cand S Q) = TWL_State_Cand (raw_cons_trail L S) Q"
-
-fun raw_prepend_trail_pq where
-"raw_prepend_trail_pq L (TWL_State_Cand S Q) = TWL_State_Cand (raw_prepend_trail L S) Q"
-
-fun update_conflicting_pq where
-"update_conflicting_pq L (TWL_State_Cand S Q) = TWL_State_Cand (update_conflicting L S) Q"
-
-lemma raw_trail_raw_cons_trail[simp]:
-  "raw_trail (raw_cons_trail L S) = L # raw_trail S"
-  by (cases S) auto
-
-lemma raw_trail_raw_prepend_trail[simp]:
-  "raw_trail (raw_prepend_trail Ls S) = Ls @ raw_trail S"
-  by (cases S) auto
-
-lemma raw_init_clss_twl_state_raw_cons_trail[simp]:
-  "raw_init_clss (twl_state (raw_cons_trail_pq L S)) = raw_init_clss (twl_state S)"
-  by (cases S) auto
-
-lemma raw_learned_clss_twl_state_raw_cons_trail[simp]:
-  "raw_learned_clss (twl_state (raw_cons_trail_pq L S)) = raw_learned_clss (twl_state S)"
-  by (cases S) auto
-
-text \<open>Useful function to chose the first non-@{term None} between two elements.\<close>
-notation Quickcheck_Exhaustive.orelse (infixr "orelse" 55)
-
-text \<open>While updating the clauses, there are several cases:
-  \<^item> if @{term L} is not watched or a conflict has already been found, then there is nothing to do;
-  \<^item> there is a literal to be watched: there are swapped;
-  \<^item> there is no literal to be watched, the other literal is not assigned: the clause
-  is a propagate candidate;
-  \<^item> there is no literal to be watched, the other literal is @{term "-L"}: the clause
-  is a tautology and nothing special is done;
-  \<^item> there is no literal to be watched, but the other literal is true: there is nothing to
-  do;
-  \<^item> there is no literal to be watched, but the other literal is false: the clause is a
-  conflict candidate.\<close>
-text \<open>We make the function slightly more general than needed:
-  \<^item> @{term removeAll} could be replace by @{term remove1}, since there are no duplicates in
-  well-founded two-watched literals.
-  \<^item> we match @{term "removeAll (-L) (watched C)"} with respect to @{term "L' # Ls'"}, while
-  @{term "[L']"} is enough.\<close>
-text \<open>The function returns a couple composed of a list of clauses and a candidate.\<close>
-fun
-  rewatch_nat_cand_single_clause ::
-  "'v literal \<Rightarrow> ('v, 'v twl_clause) ann_lits \<Rightarrow> 'v literal list twl_clause \<Rightarrow>
-   'v literal list twl_clause list \<times> 'v candidate \<Rightarrow> 'v literal list twl_clause list \<times> 'v candidate"
-where
-"rewatch_nat_cand_single_clause L M C (Cs, Ks) =
-  (if - L \<in> set (watched C) \<and> conflict Ks = None then
-     case filter (\<lambda>L'. L' \<notin> set (watched C) \<and>
-       - L' \<notin> insert L (lits_of_l (M @ get_trail_of_cand Ks))) (unwatched C) of
-       [] \<Rightarrow>
-         (case removeAll (-L) (watched C) of (* contains at most a single element *)
-             [] \<Rightarrow> (C # Cs, Prop_Or_Conf (prop_queue Ks) (Some C))
-           | L' # _ \<Rightarrow>
-             if undefined_lit (get_trail_of_cand Ks @ M) L' \<and> atm_of L \<noteq> atm_of L'
-             then (C # Cs, Prop_Or_Conf ((L', C) # prop_queue Ks) (conflict Ks))
-             else
-               (if -L' \<in> lits_of_l (get_trail_of_cand Ks @ M)
-               then (C # Cs, Prop_Or_Conf (prop_queue Ks) (conflict Ks orelse Some C))
-               else (C # Cs, Ks)))
-     | L' # _ \<Rightarrow>
-       (TWL_Clause (L' # remove1 (-L) (watched C)) (-L # remove1 L' (unwatched C)) # Cs, Ks)
-  else
-    (C # Cs, Ks))"
-
-declare rewatch_nat_cand_single_clause.simps[simp del]
-
-text \<open>We do no check if the structural invariants about the 2-WL clauses holds. Otherwise,
-  @{term "raw_trail U @ get_trail_of_cand (Prop_Or_Conf Q D) \<Turnstile>a clause C"} would work to and
-  would be a better definition.\<close>
-fun \<mu>TWL where
-"\<mu>TWL (TWL_State_Cand U K) =
-  card {L \<in> atms_of_mm (twl.clauses U). L \<notin> atm_of ` lits_of_l (raw_trail U @ get_trail_of_cand K)}"
-
-lemma get_all_mark_of_propagated_get_trail_cond[simp]:
-  "get_all_mark_of_propagated (get_trail_of_cand K) = map snd (prop_queue K)"
-proof -
-  obtain Q D where K: "K = Prop_Or_Conf Q D" by (cases K)
-  show ?thesis unfolding K by (induction Q) auto
-qed
-
-text \<open>This function could be optimised: once a conflict has been found, we could stop going through
-  the list and directly prepend all elements.\<close>
-fun rewatch_nat_cand_clss ::
-  "'v literal \<Rightarrow> ('v, 'v twl_clause) ann_lits \<Rightarrow>
-    'v twl_clause list \<times> 'v candidate \<Rightarrow>
-     'v twl_clause list  \<times> 'v candidate"
-where
-"rewatch_nat_cand_clss L M (Cs, Ks) = foldr (rewatch_nat_cand_single_clause L M) Cs ([], Ks)"
-
-declare rewatch_nat_cand_clss.simps[simp del]
-
-lemma struct_wf_rewatch_nat_cand_single_clause_cases[consumes 1, case_names wf lit_notin propagate
-  conflict no_conflict update_cls]:
-  assumes
-    wf: "struct_wf_twl_cls C" and
-    lit_notin: "-L \<notin> set (watched C) \<or> conflict Ks \<noteq> None \<Longrightarrow>
-      rewatch_nat_cand_single_clause L M C (Cs, Ks) = (C # Cs, Ks) \<Longrightarrow>
-      P"
-      and
-    single_lit_watched: "
-      -L \<in> set (watched C) \<Longrightarrow> conflict Ks = None \<Longrightarrow>
-      filter (\<lambda>L'. L' \<notin> set (watched C) \<and>
-        - L' \<notin> insert L (lits_of_l (M @ get_trail_of_cand Ks))) (unwatched C) = [] \<Longrightarrow>
-      watched C = [-L] \<Longrightarrow>
-      set (unwatched C) \<subseteq> {-L} \<Longrightarrow> conflict Ks = None \<Longrightarrow>
-      rewatch_nat_cand_single_clause L M C (Cs, Ks) =
-        (C # Cs, Prop_Or_Conf (prop_queue Ks) (Some C)) \<Longrightarrow>
-      P"
-      and
-    propagate: "\<And>L'. -L \<in> set (watched C) \<Longrightarrow> conflict Ks = None \<Longrightarrow>
-      filter (\<lambda>L'. L' \<notin> set (watched C) \<and>
-        - L' \<notin> insert L (lits_of_l (M @ get_trail_of_cand Ks))) (unwatched C) = [] \<Longrightarrow>
-      set (watched C) = {-L, L'} \<Longrightarrow>
-      undefined_lit (get_trail_of_cand Ks @ M) L' \<Longrightarrow>
-      atm_of L \<noteq> atm_of L' \<Longrightarrow>
-      rewatch_nat_cand_single_clause L M C (Cs, Ks) =
-        (C # Cs, Prop_Or_Conf ((L', C) # prop_queue Ks) (conflict Ks)) \<Longrightarrow>
-      P"
-      and
-    conflict: "\<And>L'. -L \<in> set (watched C) \<Longrightarrow> conflict Ks = None \<Longrightarrow>
-      filter (\<lambda>L'. L' \<notin> set (watched C) \<and>
-        - L' \<notin> insert L (lits_of_l (M @ get_trail_of_cand Ks))) (unwatched C) = [] \<Longrightarrow>
-      set (watched C) = {-L, L'} \<Longrightarrow>
-      -L' \<in> insert L (lits_of_l (get_trail_of_cand Ks @ M)) \<Longrightarrow>
-      rewatch_nat_cand_single_clause L M C (Cs, Ks) =
-        (C # Cs, Prop_Or_Conf (prop_queue Ks) (Some C)) \<Longrightarrow>
-      P"
-      and
-    no_conflict: "\<And>L'. -L \<in> set (watched C) \<Longrightarrow> conflict Ks = None \<Longrightarrow>
-      filter (\<lambda>L'. L' \<notin> set (watched C) \<and>
-        - L' \<notin> insert L (lits_of_l (M @ get_trail_of_cand Ks))) (unwatched C) = [] \<Longrightarrow>
-      set (watched C) = {-L, L'} \<Longrightarrow>
-      L' \<in> insert L (lits_of_l (get_trail_of_cand Ks @ M)) \<Longrightarrow>
-      rewatch_nat_cand_single_clause L M C (Cs, Ks) = (C # Cs, Ks) \<Longrightarrow>
-      P"
-      and
-    update_cls: "\<And>L' fUW. -L \<in> set (watched C) \<Longrightarrow>
-      filter (\<lambda>L'. L' \<notin> set (watched C) \<and>
-        - L' \<notin> insert L (lits_of_l (M @ get_trail_of_cand Ks))) (unwatched C) = L' # fUW
-        \<Longrightarrow>
-      rewatch_nat_cand_single_clause L M C (Cs, Ks) =
-        (TWL_Clause (L' # remove1 (-L) (watched C)) (-L # remove1 L' (unwatched C)) # Cs, Ks) \<Longrightarrow>
-      P"
-  shows P
-proof -
-  show ?thesis
-    proof (cases "- L \<notin> set (watched C) \<or> conflict Ks \<noteq> None")
-      case l: True
-      then show ?thesis
-        apply - by (rule lit_notin) (auto simp add: rewatch_nat_cand_single_clause.simps)
-    next
-      case False
-      then have L: "- L \<in> set (watched C)" and [simp]: "conflict Ks = None"
-        by auto
-      show ?thesis
-        proof (cases "filter (\<lambda>L'. L' \<notin> set (watched C) \<and>
-          - L' \<notin> insert L (lits_of_l (M @ get_trail_of_cand Ks)))
-          (unwatched C)")
-          case (Cons L' fUW)
-          then show ?thesis
-            apply - by (rule update_cls) (auto simp add: rewatch_nat_cand_single_clause.simps L)
-        next
-          case filter: Nil
-          then show ?thesis
-            proof (cases "remove1 (-L) (watched C)")
-              case Nil
-              then show ?thesis apply -
-                apply (rule single_lit_watched; cases C)
-                using wf L filter by (auto simp: rewatch_nat_cand_single_clause.simps length_list_2
-                  remove1_Nil)
-            next
-              case (Cons L' fW)
-              then have dist: "distinct (watched C)" and l_W: "length (watched C) \<le> 2"
-                using wf by (cases C, auto)+
-              then have [simp]: "fW = []" using Cons
-                by (metis L One_nat_def Suc_1 Suc_eq_plus1 add_diff_cancel_left' add_right_imp_eq
-                  diff_is_0_eq le_Suc_eq length_0_conv length_remove1 list.distinct(1) list.size(4))
-              then have C: "set (watched C) = {-L, L'}"
-                using l_W L dist arg_cong[OF Cons, of set, simplified] by auto
-              have [simp]: "\<And>L'. removeAll L' (watched C) = remove1 L' (watched C)"
-                using dist by (simp add: distinct_remove1_removeAll)
-              have [simp]: "remove1 L' (watched C) \<noteq> [L']"
-                by (metis DiffD2 dist insertI1 list.simps(15) set_remove1_eq)
-              show ?thesis
-                apply (cases "undefined_lit (get_trail_of_cand Ks @ M) L'\<and> atm_of L \<noteq> atm_of L' ")
-                apply (rule propagate)
-                  using L filter C Cons dist
-                  apply (auto simp: rewatch_nat_cand_single_clause.simps atm_of_eq_atm_of)[7]
-                apply (cases "-L' \<in> insert L (lits_of_l (get_trail_of_cand Ks @ M))")
-                apply (rule conflict)
-                  using L filter C Cons apply (auto simp: rewatch_nat_cand_single_clause.simps L
-                    Quickcheck_Exhaustive.orelse_def)[6]
-                  apply (rule no_conflict)
-                  using L filter C Cons apply (auto simp: rewatch_nat_cand_single_clause.simps
-                    defined_lit_map lits_of_def image_Un atm_of_eq_atm_of image_image
-                    rev_image_eqI)[6]
-                done
-            qed
-        qed
-    qed
-qed
-
-lemma wf_twl_cls_struct_wf_twl_cls: "wf_twl_cls M C \<Longrightarrow> struct_wf_twl_cls C"
-  by (cases C) auto
-
-lemmas wf_rewatch_nat_cand_single_clause_cases =
-  struct_wf_rewatch_nat_cand_single_clause_cases[OF wf_twl_cls_struct_wf_twl_cls]
-
-lemma prop_queue_rewatch_nat_cand_single_clause_eq_or_cons:
-  "prop_queue (snd (rewatch_nat_cand_single_clause L M C S)) = prop_queue (snd S) \<or>
-  (\<exists>L'. prop_queue (snd (rewatch_nat_cand_single_clause L M C S)) = L' # prop_queue (snd S))"
-  apply (cases C, cases S)
-  apply (auto simp: raw_clause_def filter_empty_conv true_annots_true_cls_def_iff_negation_in_model
-    comp_def rewatch_nat_cand_single_clause.simps lits_of_def image_image split: list.splits
-     simp del: watched_only_lazy_updates.simps)
-  done
-
-lemma lit_of_case_Propagated[simp]: "lit_of (case x of (x, xa) \<Rightarrow> Propagated x xa) = fst x"
-  by (cases x) auto
-
-lemma prop_queue_first_is_undefined:
-  assumes "prop_queue (snd (rewatch_nat_cand_single_clause L M C S)) = L' # prop_queue (snd S)"
-  shows
-    "undefined_lit (get_trail_of_cand (snd S) @ M) (fst L')" and
-    "snd L' = C" and
-    "fst L' \<in># clause C" and
-    "fst L' \<noteq> -L" and
-    "fst L' \<noteq> L"
-        using assms
-          apply (cases C, cases S)
-          apply (auto simp: rewatch_nat_cand_single_clause.simps
-            split: list.splits if_splits
-            simp del: watched_only_lazy_updates.simps)
-        using assms
-        apply (cases C, cases S)
-        apply (auto simp: rewatch_nat_cand_single_clause.simps
-          split: list.splits if_splits
-          simp del: watched_only_lazy_updates.simps)
-      using assms
-      apply (cases C, cases S)
-      apply (auto simp: rewatch_nat_cand_single_clause.simps clause_def raw_clause_def
-        split: list.splits if_splits
-        simp del: watched_only_lazy_updates.simps
-        dest!: arg_cong[of "removeAll _ _" _ set])
-      using assms
-    apply (cases C, cases S)
-    apply (auto simp: rewatch_nat_cand_single_clause.simps clause_def raw_clause_def
-      split: list.splits if_splits
-      simp del: watched_only_lazy_updates.simps
-      dest!: arg_cong[of "removeAll _ _" _ set])
-    using assms
-  apply (cases C, cases S)
-  apply (auto simp: rewatch_nat_cand_single_clause.simps clause_def raw_clause_def
-    split: list.splits if_splits
-    simp del: watched_only_lazy_updates.simps
-    dest!: arg_cong[of "removeAll _ _" _ set])
-  done
-
-lemmas rewatch_nat_cand_single_clause_cases =
-  wf_rewatch_nat_cand_single_clause_cases[OF wf_twl_cls_append[of "get_trail_of_cand _"],
-    consumes 2, case_names wf lit_notin propagate conflict no_conflict update_cls]
-
-fun rewatch_nat_cand :: "'a literal \<Rightarrow> 'a twl_state_cands \<Rightarrow> 'a twl_state_cands"  where
-"rewatch_nat_cand L (TWL_State_Cand S Ks) =
-  (let
-    (N, K) = rewatch_nat_cand_clss L (raw_trail S) (raw_init_clss S, Ks);
-    (U, K') = rewatch_nat_cand_clss L (raw_trail S) (raw_learned_clss S, K) in
-  TWL_State_Cand
-    (TWL_State (raw_trail S) N U (backtrack_lvl S) (raw_conflicting S))
-    K')"
-
-lemma rewatch_nat_cand_single_clause_hd:
-  "raw_clss_l (fst (rewatch_nat_cand_single_clause L M C K)) =
-      raw_clss_l ((C # (fst K)))"
-  apply (cases C, cases K)
-  apply (auto simp: raw_clause_def filter_empty_conv true_annots_true_cls_def_iff_negation_in_model
-    comp_def rewatch_nat_cand_single_clause.simps lits_of_def image_image
-    clause_def
-    split: list.splits
-     simp del: watched_only_lazy_updates.simps)
-  apply (auto dest: filter_in_list_prop_verifiedD simp: multiset_eq_iff)
-  done
-
-lemma rewatch_nat_cand_single_clause_clauses:
-  "raw_clss_l (fst (rewatch_nat_cand_clss L M (N, Ks))) = raw_clss_l N"
-  by (induction N) (simp_all add: rewatch_nat_cand_clss.simps
-    rewatch_nat_cand_single_clause_hd[simplified])
-
-fun undefined_lit_list :: "('a literal \<times> 'a twl_clause) list
-   \<Rightarrow> ('a, 'a twl_clause) ann_lits \<Rightarrow> bool" where
-"undefined_lit_list [] _ \<longleftrightarrow> True" |
-"undefined_lit_list (L # Ls) M \<longleftrightarrow> undefined_lit (map (case_prod Propagated) Ls @ M) (fst L) \<and>
-  undefined_lit_list Ls M"
-
-lemma undefined_lit_list_append[simp]:
-  "undefined_lit_list (Ls @ Ls') M \<longleftrightarrow>
-    undefined_lit_list Ls (map (case_prod Propagated) Ls' @ M) \<and>
-    undefined_lit_list Ls' M"
-  by (induction Ls) auto
-
-lemma prop_queue_rewatch_nat_cand_clss_eq_or_cons:
-  "\<exists>L'. prop_queue (snd (rewatch_nat_cand_clss L M K)) = L' @ prop_queue (snd K)
-  \<and> undefined_lit_list L' (get_trail_of_cand (snd K) @ M)
-  \<and> (\<forall>(l, C) \<in> set L'. C \<in> set (fst K) \<and> l \<in># clause C \<and> l \<noteq> -L \<and> l \<noteq> L)" (is "\<exists>L'. ?P K L'")
-proof -
-  obtain Cs Q where K: "K = (Cs, Q)"
-    by (cases K)
-  show ?thesis
-    unfolding K
-    proof (induction Cs)
-      case Nil
-      then show ?case
-       by (auto simp: rewatch_nat_cand_clss.simps)[]
-    next
-      case (Cons C Cs)
-      then obtain L' where
-        L': "prop_queue (snd (rewatch_nat_cand_clss L M (Cs, Q))) = L' @ prop_queue (snd (Cs, Q))"
-          and
-        undef: "undefined_lit_list L' (get_trail_of_cand (snd (Cs, Q)) @ M)" and
-        aL': "\<forall>a\<in>set L'. case a of (l, C) \<Rightarrow> C \<in> set (fst (Cs, Q)) \<and> l \<in># clause C \<and> l \<noteq> -L \<and>
-          l \<noteq> L"
-        by fast
-      consider
-          (Nil) "prop_queue (snd (rewatch_nat_cand_single_clause L M C
-             (foldr (rewatch_nat_cand_single_clause L M) Cs ([], Q)))) =
-           prop_queue (snd (foldr (rewatch_nat_cand_single_clause L M) Cs ([], Q)))"
-        | (Cons) L'' where
-          "prop_queue (snd (rewatch_nat_cand_single_clause L M C
-             (foldr (rewatch_nat_cand_single_clause L M) Cs ([], Q)))) =
-           L'' # prop_queue (snd (foldr (rewatch_nat_cand_single_clause L M) Cs ([], Q)))"
-        using prop_queue_rewatch_nat_cand_single_clause_eq_or_cons[of L M C
-         "foldr (rewatch_nat_cand_single_clause L M) Cs ([], Q)"] by blast
-    then show ?case
-      proof cases
-        case Nil
-        then show ?thesis
-          using L' undef aL' by (auto simp: rewatch_nat_cand_clss.simps)[]
-      next
-        case (Cons L'')
-        then show ?thesis
-          using L' undef aL'  prop_queue_first_is_undefined[of L M C
-           "foldr (rewatch_nat_cand_single_clause L M) Cs ([], Q)" L'']
-          by (auto simp: rewatch_nat_cand_clss.simps)
-      qed
-    qed
-qed
-
-lemma prop_queue_rewatch_nat_cand_eq_or_cons:
-  "\<exists>L'. prop_queue (cand (rewatch_nat_cand L S)) = L' @ prop_queue (cand S)
-  \<and> undefined_lit_list L' (get_trail_of_cand (cand S) @ raw_trail (twl_state S))
-  \<and> (\<forall>(l, C) \<in> set L'. C \<in> set (raw_clauses (twl_state S)) \<and> l \<in># clause C
-    \<and> l \<noteq> -L \<and> l \<noteq> L)"
-proof -
-  obtain T Ks where S: "S = TWL_State_Cand T Ks"
-    by (cases S)
-  obtain U K' where
-    U: "rewatch_nat_cand_clss L (raw_trail T) (raw_init_clss T, Ks) = (U, K')"
-    (is "?H = _") by (cases ?H)
-
-  obtain V K'' where
-    V: "rewatch_nat_cand_clss L (raw_trail T) (raw_learned_clss T, K') = (V, K'')"
-    (is "?H = _") by (cases ?H)
-
-  show ?thesis unfolding S
-    using prop_queue_rewatch_nat_cand_clss_eq_or_cons[of L "raw_trail T" "(raw_init_clss T, Ks)"]
-    using prop_queue_rewatch_nat_cand_clss_eq_or_cons[of L "raw_trail T" "(raw_learned_clss T, K')"]
-    by (auto simp: comp_def U V)
-qed
-
-lemma twl_clauses_rewatch_nat_cand[simp]:
-  "twl.clauses (twl_state (rewatch_nat_cand L S)) = twl.clauses (twl_state S)"
-proof -
-  obtain T Ks where S: "S = TWL_State_Cand T Ks"
-    by (cases S)
-  obtain U K' where
-    U: "rewatch_nat_cand_clss L (raw_trail T) (raw_init_clss T, Ks) = (U, K')"
-    (is "?H = _") by (cases ?H)
-
-  obtain V K'' where
-    V: "rewatch_nat_cand_clss L (raw_trail T) (raw_learned_clss T, K') = (V, K'')"
-    (is "?H = _") by (cases ?H)
-
-  have "mset (map clause U) = mset (map clause (raw_init_clss T))"
-    using rewatch_nat_cand_single_clause_clauses[of L "raw_trail T" "raw_init_clss T"
-      "Ks"] by (auto simp: comp_def U clause_def raw_clause_def clause_def_lambda)
-  moreover have "mset (map clause V) = mset (map clause
-  (raw_learned_clss T))"
-    using rewatch_nat_cand_single_clause_clauses[of L "raw_trail T" "raw_learned_clss T"
-      "K'"] by (auto simp: comp_def V clause_def_lambda raw_clause_def)
-  ultimately show ?thesis  unfolding S
-    by (auto simp: comp_def raw_clauses_def U V clause_def raw_clause_def)
-qed
-
-lemma true_annot_mono_append_append:
-  "A @ C \<Turnstile>a D \<Longrightarrow> A @ B @ C \<Turnstile>a D"
-  "A @ C \<Turnstile>a D \<Longrightarrow> L # A @ B @ C \<Turnstile>a D"
-  by (rule true_annot_mono; auto)+
-
-lemma true_annot_mono':
-  "\<not>I' \<Turnstile>a N \<Longrightarrow> I \<Turnstile>a N \<Longrightarrow> \<not>set I \<subseteq> set I' "
-  using true_annot_mono by blast
-
-lemma prop_queue_cand_raw_cons_trail[simp]:
-  "prop_queue (cand (raw_cons_trail_pq (Propagated L C') S)) = prop_queue (cand S)"
-  by (cases S) auto
-
-lemma \<mu>TWL_Prop_Or_Conf_append_raw_cons_trail:
-  "\<mu>TWL (TWL_State_Cand S (Prop_Or_Conf (l @ [(L, C')]) D)) =
-    \<mu>TWL (TWL_State_Cand (raw_cons_trail (Propagated L C') S) (Prop_Or_Conf l D))"
-  by (auto simp: comp_def)
-
-lemma get_all_mark_of_propagated_map_Propagated[simp]:
-  "get_all_mark_of_propagated (map (\<lambda>(x, y). Propagated x y) Q) = map snd Q"
-  by (induction Q) auto
-
-lemma YYY:
-  "\<mu>TWL (raw_cons_trail_pq (Propagated L C')
-    (rewatch_nat_cand L (TWL_State_Cand S (Prop_Or_Conf Q D))))
-   \<le> \<mu>TWL (TWL_State_Cand S (Prop_Or_Conf (Q @ [(L, C')]) D))"
-proof -
-  obtain U K' where
-    U: "rewatch_nat_cand_clss L (raw_trail S) (raw_init_clss S, Prop_Or_Conf Q D) = (U, K')"
-    (is "?H = _") by (cases ?H)
-
-  obtain V K'' where
-    V: "rewatch_nat_cand_clss L (raw_trail S) (raw_learned_clss S, K') = (V, K'')"
-    (is "?H = _") by (cases ?H)
-
-  obtain Q'' D'' where K'': "K'' = Prop_Or_Conf Q'' D''"
-    by (cases K'')
-  obtain P where P: "Q'' = P @ Q"
-    using prop_queue_rewatch_nat_cand_eq_or_cons[of L "TWL_State_Cand S (Prop_Or_Conf Q D)"]
-    by (auto simp: comp_def U V K'')
-
-  have H1: "set_mset (mset (map clause U)) =
-    clause ` set_mset (mset (raw_init_clss S))"
-    using rewatch_nat_cand_single_clause_clauses[of L "raw_trail S" "raw_init_clss S"
-      "Prop_Or_Conf Q D"] by (auto simp: comp_def U clause_def_lambda)
-  moreover
-    have H2: "set_mset (mset (map clause V)) =
-      clause ` set_mset (mset (raw_learned_clss S))"
-      using rewatch_nat_cand_single_clause_clauses[of L "raw_trail S" "raw_learned_clss S"
-        "K'"] by (auto simp: comp_def V clause_def_lambda)
-  show ?thesis
-    using H1 H2
-    by (auto simp: comp_def U V K'' image_Un P (* raw_clause_def *)
-      clause_def image_image lits_of_def intro!: Nat.diff_le_mono2 card_mono)
-qed
-
-text \<open>This purely technical lemma states that if there is no new defined literals, then @{term Ls}
-  is empty.\<close>
-lemma \<mu>TWL_eq_no_new_propagated_lit:
-  assumes
-    c: "card {La \<in> atms_of_ms (clause ` set (raw_clauses S)).
-      La \<noteq> atm_of L \<and> La \<notin> (\<lambda>x. atm_of (lit_of x)) ` set (raw_trail S) \<and>
-      La \<notin> (\<lambda>x. atm_of (fst x)) ` set Ls \<and>
-      La \<notin> (\<lambda>x. atm_of (fst x)) ` set l} =
-    card {La \<in> atms_of_ms (clause ` set (raw_clauses S)).
-      La \<noteq> atm_of L \<and> La \<notin> (\<lambda>x. atm_of (lit_of x)) ` set (raw_trail S) \<and>
-      La \<notin> (\<lambda>x. atm_of (fst x)) ` set l}" and
-    undef: "undefined_lit_list Ls (map (\<lambda>(x, y). Propagated x y) l @ raw_trail S)" and
-    C: "\<forall>(l, C)\<in>set Ls. C \<in> set (raw_clauses S) \<and> l \<in># clause C \<and> l \<noteq> - L \<and> l \<noteq> L"
-  shows "Ls = []"
-proof (rule ccontr)
-  assume "Ls \<noteq> []"
-  then obtain L' C' Ls' where Ls: "Ls = (L', C') # Ls'"
-    by (cases Ls) auto
-  let ?D =" {La \<in> atms_of_ms (clause ` set (raw_clauses S)).
-      La \<noteq> atm_of L \<and> La \<notin> (\<lambda>x. atm_of (lit_of x)) ` set (raw_trail S) \<and>
-      La \<notin> (\<lambda>x. atm_of (fst x)) ` set Ls \<and>
-      La \<notin> (\<lambda>x. atm_of (fst x)) ` set l}"
-  let ?C = " {La \<in> atms_of_ms (clause ` set (raw_clauses S)).
-      La \<noteq> atm_of L \<and> La \<notin> (\<lambda>x. atm_of (lit_of x)) ` set (raw_trail S) \<and>
-      La \<notin> (\<lambda>x. atm_of (fst x)) ` set l}"
-  have "?D \<subseteq> ?C"
-    by blast
-  moreover have "finite ?D"
-    by auto
-  ultimately have "?D = ?C"
-    by (simp add: c card_subset_eq)
-  then have H: "\<And>La. La \<in> atms_of_ms (clause ` set (raw_clauses S)) \<Longrightarrow>
-    La \<noteq> atm_of L \<Longrightarrow> La \<notin> (\<lambda>x. atm_of (lit_of x)) ` set (raw_trail S) \<Longrightarrow>
-    La \<notin> (\<lambda>x. atm_of (fst x)) ` set l \<Longrightarrow>
-    La \<notin> (\<lambda>x. atm_of (fst x)) ` set Ls"
-    by blast
-  have undef: "undefined_lit
-    (map (\<lambda>(x, y). Propagated x y) Ls' @ map (\<lambda>(x, y). Propagated x y) l @ raw_trail S) L'"
-    using undef unfolding Ls by auto
-  have C': "C' \<in> set (raw_clauses S)" and "L' \<in># clause C'" and LL': "L' \<noteq> -L" "L' \<noteq> L"
-    using C unfolding Ls by auto
-  then have "atm_of L' \<in> atms_of_ms (clause ` set (raw_clauses S))"
-    by (simp add: C' in_implies_atm_of_on_atms_of_ms)
-  moreover have "atm_of L' \<noteq> atm_of L"
-    using LL' by (auto simp: atm_of_eq_atm_of)
-  moreover have "atm_of L' \<notin> (\<lambda>x. atm_of (lit_of x)) ` set (raw_trail S)" and
-    "atm_of L' \<notin> (\<lambda>x. atm_of (fst x)) ` set l"
-    using undef by (auto simp: defined_lit_map image_Un image_image)
-  moreover have "atm_of L' \<in> (\<lambda>x. atm_of (fst x)) ` set Ls"
-    unfolding Ls by auto
-  ultimately show False using H[of "atm_of L'"] by fast
-qed
-
-text \<open>Remark that:
-  \<^item> we do not change the conflicting clause, once one has been found. It should be possible
-  to take the shorter of the conflicts with respect to the trail.
-  \<close>
-function do_propagate_or_conflict_step :: "'a twl_state_cands \<Rightarrow> 'a twl_state_cands" where
-"do_propagate_or_conflict_step (TWL_State_Cand S (Prop_Or_Conf Q (Some D))) =
-  update_conflicting_pq (Some (raw_clause D))
-    (TWL_State_Cand (raw_prepend_trail (get_trail_of_cand (Prop_Or_Conf Q (Some D))) S)
-      (Prop_Or_Conf [] None))" |
-"do_propagate_or_conflict_step (TWL_State_Cand S (Prop_Or_Conf [] None)) =
-  TWL_State_Cand S (Prop_Or_Conf [] None)" |
-"do_propagate_or_conflict_step (TWL_State_Cand S (Prop_Or_Conf (l @ [(L, C')]) None)) =
-  (do_propagate_or_conflict_step
-    (raw_cons_trail_pq (Propagated L C')
-      (rewatch_nat_cand L (TWL_State_Cand S (Prop_Or_Conf l None)))))"
-  apply (rename_tac P x)
-  apply (case_tac x, case_tac "cand x"; case_tac "conflict (cand x)";
-    case_tac "prop_queue (cand x)" rule: rev_cases; simp)
-  by auto
-termination
-  apply (relation "{(T, S).
-    ([\<mu>TWL T, length (prop_queue (cand T))], [\<mu>TWL S, length (prop_queue (cand S))])
-    \<in> lexn less_than 2}")
-proof (goal_cases)
-  case 1
-  show ?case by (auto simp: wf_lexn intro!: wf_if_measure_f)
-next
-  case (2 S l L C')
-  obtain T Q' where T: "rewatch_nat_cand L (TWL_State_Cand S (Prop_Or_Conf l None)) =
-    TWL_State_Cand T Q'"
-    by (cases "rewatch_nat_cand L (TWL_State_Cand S (Prop_Or_Conf l None))")
-  have ST: "clause ` set (raw_clauses T) =
-    clause ` set (raw_clauses S)"
-    using twl_clauses_rewatch_nat_cand[of L "TWL_State_Cand S (Prop_Or_Conf l None)"]
-    unfolding T
-    (* TODO tune proof *)
-    apply (auto simp: comp_def image_Un
-          simp del: rewatch_nat_cand.simps)
-    apply (metis (no_types, lifting) Un_iff image_eqI set_append set_map set_mset_mset union_code)+
-    done
-  have [simp]: "raw_trail T = raw_trail S"
-    using T by (auto split: Product_Type.prod.splits)
-  show ?case
-    using YYY[of L C' S l None]
-    prop_queue_rewatch_nat_cand_eq_or_cons[of L "TWL_State_Cand S (Prop_Or_Conf l None)"]
-    apply (auto simp add: comp_def lexn_n \<mu>TWL_Prop_Or_Conf_append_raw_cons_trail
-      T ST \<mu>TWL_eq_no_new_propagated_lit[of S]
-      simp del: lexn.simps(2) rewatch_nat_cand.simps
-      simp add: lits_of_def image_image image_Un)
-    done
-qed
-
-lemma no_dup_rewatch_nat_cand_single_clause:
-  fixes L :: "'v literal"
-  assumes
-    L: "L \<in> lits_of_l M" and
-    wf: "wf_twl_cls (get_trail_of_cand Ks @ M) C" and
-    n_d: "no_dup (get_trail_of_cand Ks @ M)"
-  shows "no_dup (M @ get_trail_of_cand (snd (rewatch_nat_cand_single_clause L M C (Cs, Ks))))"
-  using n_d wf apply (cases rule: rewatch_nat_cand_single_clause_cases[of Ks M C L Ks M Cs])
-  using L n_d by (auto simp: defined_lit_map comp_def image_image image_Un)
-
-lemma wf_twl_cls_prop_in_trailD:
-  assumes "wf_twl_cls M (TWL_Clause W UW)"
-  shows "\<forall>L \<in> set W. -L \<in> lits_of_l M \<longrightarrow> (\<forall>L' \<in> set UW. L' \<notin> set W \<longrightarrow> -L' \<in> lits_of_l M)"
-  using assms by auto
-
-lemma rewatch_nat_cand_single_clause_conflict:
-  assumes
-    L: "L \<in> lits_of_l M" and
-    wf: "wf_twl_cls (get_trail_of_cand Ks @ M) C" and
-    conf: "conflict Ks = Some D" and
-    conf': "conflict (snd (rewatch_nat_cand_single_clause L M C (Cs, Ks))) = Some D'" and
-    n_d: "no_dup (get_trail_of_cand Ks @ M)" and
-    confI: "get_trail_of_cand Ks @ M \<Turnstile>as CNot (clause D)"
-  shows "get_trail_of_cand Ks @ M \<Turnstile>as CNot (clause D')"
-  apply (cases C)
-  using n_d wf apply (cases rule: rewatch_nat_cand_single_clause_cases[of Ks M C L Ks M Cs])
-  prefer 4
-    using conf conf' confI L
-    apply (auto simp add: raw_clause_def true_annots_true_cls_def_iff_negation_in_model
-      lits_of_def image_image image_Un Quickcheck_Exhaustive.orelse_def
-        simp del: watched_only_lazy_updates.simps wf_twl_cls.simps
-        dest!: wf_twl_cls_prop_in_trailD)[]
-  using conf conf' confI L
-  apply (auto simp add: raw_clause_def  true_annots_true_cls_def_iff_negation_in_model
-    Quickcheck_Exhaustive.orelse_def
-      simp del: watched_only_lazy_updates.simps
-    )[5]
-  done
-
-lemma rewatch_nat_cand_single_clause_conflict_found:
-  assumes
-    L: "L \<in> lits_of_l M" and
-    wf: "wf_twl_cls (get_trail_of_cand Ks @ M) C" and
-    n_d: "no_dup (get_trail_of_cand Ks @ M)" and
-    conf: "conflict Ks = None" and
-    conf': "conflict (snd (rewatch_nat_cand_single_clause L M C (Cs, Ks))) = Some D'"
-  shows "get_trail_of_cand Ks @ M \<Turnstile>as CNot (clause D')"
-  apply (cases C)
-  using n_d wf apply (cases rule: rewatch_nat_cand_single_clause_cases[of Ks M C L Ks M Cs])
-  using conf conf' L
-  (* TODO tune proof *)
-  apply (auto simp: raw_clause_def filter_empty_conv true_annots_true_cls_def_iff_negation_in_model
-    Quickcheck_Exhaustive.orelse_def lits_of_def image_image image_Un clause_def
-     simp del: watched_only_lazy_updates.simps)
-  apply force+
-  done
-
-lemma rewatch_nat_cand_single_clause_no_dup:
-  fixes Ks :: "'v candidate" and M :: "('v, 'v twl_clause) ann_lits"
-  and L :: "'v literal" and Cs :: "'v twl_clause list" and C :: "'v twl_clause"
-  defines "S \<equiv> rewatch_nat_cand_single_clause L M C (Cs, Ks)"
-  assumes wf: "wf_twl_cls M C" and
-    n_d: "no_dup (get_trail_of_cand Ks @ M)" and
-    undef: "undefined_lit (get_trail_of_cand Ks @ M) L"
-  shows "no_dup (get_trail_of_cand (snd S) @ M)"
-  using wf n_d apply (cases rule: wf_rewatch_nat_cand_single_clause_cases[of M C L Ks M Cs])
-  using undef unfolding S_def by (auto simp add: defined_lit_map image_Un image_image comp_def)
-
-text \<open>The full invariant does not hold while running @{term "do_propagate_or_conflict_step"}:
-  the data structure is only partly well-founded.\<close>
-primrec watched_wf_twl_cls_pq :: "('a, 'b) ann_lits \<Rightarrow> 'a literal list \<Rightarrow> 'a twl_clause \<Rightarrow>
-  bool" where
-"watched_wf_twl_cls_pq M Q (TWL_Clause W UW) \<longleftrightarrow>
-   (\<forall>L \<in> set W. -L \<in> lits_of_l M \<longrightarrow> (\<forall>L' \<in> set UW. L' \<notin> set (W @ Q) \<longrightarrow> -L' \<in> lits_of_l M))"
-
-primrec wf_twl_cls_pq :: "('v, 'mark) ann_lits \<Rightarrow> 'v literal list \<Rightarrow> 'v twl_clause \<Rightarrow>
-  bool" where
-"wf_twl_cls_pq M Q (TWL_Clause W UW) \<longleftrightarrow>
-   struct_wf_twl_cls (TWL_Clause W UW) \<and> watched_wf_twl_cls_pq M Q (TWL_Clause W UW) \<and>
-   watched_only_lazy_updates M (TWL_Clause W UW)"
-
-definition wf_twl_state_pq :: "'v twl_state_cands \<Rightarrow> bool" where
-"wf_twl_state_pq S \<longleftrightarrow>
-  (\<forall>C \<in> set (raw_clauses (twl_state S)).
-    wf_twl_cls_pq (raw_trail (twl_state S)) (map fst (prop_queue (cand S))) C) \<and>
-    no_dup (raw_trail (twl_state S) @ get_trail_of_cand (cand S))"
-
-lemma twl_raw_clauses_update_conflicting[simp]:
-  "raw_clauses (update_conflicting D S) = raw_clauses S"
-  unfolding raw_clauses_def by auto
-
-lemma wf_twl_state_pq_TWL_State_Cand_update_conflicting:
-  "wf_twl_state_pq (TWL_State_Cand (update_conflicting D S) Q) \<longleftrightarrow>
-   wf_twl_state_pq (TWL_State_Cand S Q)"
-  unfolding wf_twl_state_pq_def by (auto simp del: wf_twl_cls_pq.simps simp: comp_def)
-
-lemma wf_twl_state_pq_conflicting_Some_None:
-  "wf_twl_state_pq (TWL_State_Cand S (Prop_Or_Conf [] (Some D))) \<longleftrightarrow>
-  wf_twl_state_pq (TWL_State_Cand S (Prop_Or_Conf [] None))"
-  unfolding wf_twl_state_pq_def by (auto simp del: wf_twl_cls_pq.simps simp: comp_def)
-
-lemma struct_wf_twl_cls_rewatch_nat_cand_clss:
-  assumes "\<forall>x\<in>set Cs. struct_wf_twl_cls x"
-  shows "\<forall>x\<in>set (fst (rewatch_nat_cand_clss L M (Cs, Ks))). struct_wf_twl_cls x"
-  using assms
-proof (induction Cs)
-  case Nil
-  then show ?case by (auto simp: rewatch_nat_cand_clss.simps)
-next
-  case (Cons C Cs)
-  then show ?case
-  apply (cases "foldr (rewatch_nat_cand_single_clause L M) Cs ([], Ks)")
-  apply (cases C)
-    apply (cases "rewatch_nat_cand_single_clause L M C (foldr (rewatch_nat_cand_single_clause L M)
-      Cs ([], Ks))";
-      cases "snd (rewatch_nat_cand_single_clause L M C (foldr (rewatch_nat_cand_single_clause L M)
-      Cs ([], Ks)))")
-  by (auto simp: rewatch_nat_cand_clss.simps rewatch_nat_cand_single_clause.simps lits_of_def
-    image_image image_Un length_list_2
-    split: if_splits list.splits
-    dest!: filter_eq_ConsD)[]
-qed
-
-lemma struct_wf_twl_cls_rewatch_nat_cand:
-  assumes wf: "\<forall>x\<in>set (raw_clauses T). struct_wf_twl_cls x"
-  shows "\<forall>x\<in>set (raw_clauses (twl_state (raw_cons_trail_pq (Propagated L C')
-    (rewatch_nat_cand L (TWL_State_Cand T Ks))))). struct_wf_twl_cls x"
-proof -
-  obtain U K' where
-    U: "rewatch_nat_cand_clss L (raw_trail T) (raw_init_clss T, Ks) = (U, K')"
-    (is "?H = _") by (cases ?H)
-
-  obtain V K'' where
-    V: "rewatch_nat_cand_clss L (raw_trail T) (raw_learned_clss T, K') = (V, K'')"
-    (is "?H = _") by (cases ?H)
-  have "\<And>x. x \<in> set U \<Longrightarrow> struct_wf_twl_cls x"
-    using struct_wf_twl_cls_rewatch_nat_cand_clss[of "raw_init_clss T" L "raw_trail T" Ks] wf U
-    by (cases T) (auto simp: raw_clauses_def)
-
-  moreover have "\<And>x. x \<in> set V \<Longrightarrow> struct_wf_twl_cls x"
-    using struct_wf_twl_cls_rewatch_nat_cand_clss[of "raw_learned_clss T" L "raw_trail T" K'] wf V
-    by (cases T) (auto simp: raw_clauses_def)
-  ultimately show ?thesis
-    by (auto simp: raw_clauses_def Product_Type.prod.case_distrib U V)[]
-qed
-
-lemma struct_wf_twl_cls_do_propagate_or_conflict_step:
-  assumes "\<forall>C\<in>set (raw_clauses (twl_state S)). struct_wf_twl_cls C" and
-   "C \<in> set (raw_clauses (twl_state (do_propagate_or_conflict_step S)))"
-  shows "struct_wf_twl_cls C"
-  using assms
-  apply (induction S rule: do_propagate_or_conflict_step.induct)
-    apply (auto simp: Product_Type.prod.case_distrib)[]
-   apply (auto simp: Product_Type.prod.case_distrib)[]
-  by (simp del: rewatch_nat_cand.simps
-    add: struct_wf_twl_cls_rewatch_nat_cand)
-
-subsection \<open>Skip and Resolve\<close>
-fun do_analyse_step :: "'v twl_state \<Rightarrow> 'v twl_state" where
-"do_analyse_step (TWL_State (Propagated L C # Ls) N U k (Some D)) =
-  (if -L \<notin> set D
-  then TWL_State (Propagated L C # Ls) N U k (Some D)
-  else if get_maximum_level (Propagated L C # Ls) (mset (remove1 (-L) D)) = k
-  then (TWL_State Ls N U k (Some (remdups (remove1 L (raw_clause C) @ remove1 (-L) D))))
-  else (TWL_State (Propagated L C # Ls) N U k (Some D)))" |
-"do_analyse_step S = S"
-
-fun raw_tl_trail where
-"raw_tl_trail (TWL_State M N U k C) = TWL_State (tl M) N U k C"
-
-
-interpretation twl: conflict_driven_clause_learning\<^sub>W
-  clause
-  raw_clss_l "op @"
-  "\<lambda>L C. L \<in> set C" "op #" "\<lambda>C. remove1_cond (\<lambda>D. clause D = clause C)"
-
-  mset "\<lambda>xs ys. case_prod append (fold (\<lambda>x (ys, zs). (remove1 x ys, x # zs)) xs (ys, []))"
-  remove1
-
-  raw_clause "\<lambda>C. TWL_Clause [] C"
-  trail "\<lambda>S. hd (raw_trail S)"
-  raw_init_clss raw_learned_clss backtrack_lvl raw_conflicting
-
-  raw_cons_trail raw_tl_trail
-
-  apply unfold_locales apply (auto simp: hd_map comp_def map_tl ac_simps raw_clause_def
-    union_mset_list mset_map_mset_remove1_cond ex_mset_unwatched_watched clause_def)
-oops
 
 end
